src/n-bit/numeral_bitScript.sml
@@ -6,14 +6,8 @@
 (* DATE          : 2001-2005                                                 *)
 (* ========================================================================= *)
 
-(* interactive use:
-  load "bitTheory";
-*)
-
-open HolKernel Parse boolLib bossLib lcsymtacs;
-open Q arithmeticTheory numeralTheory;
-open bitTheory;
-open numposrepTheory
+open HolKernel Parse boolLib bossLib lcsymtacs
+open arithmeticTheory numeralTheory bitTheory numposrepTheory
 
 val _ = new_theory "numeral_bit";
 
@@ -32,421 +26,459 @@ val numeral_mod2 = Q.store_thm("numeral_mod2",
        `NUMERAL (BIT2 n) = 2 * (SUC n)`
        by metisLib.METIS_TAC [NUMERAL_DEF, ADD_ASSOC, ADD1, ADD, BIT2, TIMES2]]
    \\ pop_assum SUBST1_TAC
-   \\ srw_tac [numSimps.MOD_ss] []
-);
+   \\ srw_tac [numSimps.MOD_ss] [])
 
-val iDUB_NUMERAL = store_thm("iDUB_NUMERAL",
-  `numeral$iDUB (NUMERAL i) = NUMERAL (numeral$iDUB i)`,
-  REWRITE_TAC [arithmeticTheory.NUMERAL_DEF]);
+val iDUB_NUMERAL = Q.store_thm("iDUB_NUMERAL",
+   `numeral$iDUB (NUMERAL i) = NUMERAL (numeral$iDUB i)`,
+   REWRITE_TAC [arithmeticTheory.NUMERAL_DEF])
 
 val BIT_REV_def =
-  Prim_rec.new_recursive_definition
-  {name = "BIT_REV_def",
-   def = ``(BIT_REV 0 x y = y)
-        /\ (BIT_REV (SUC n) x y =
-              BIT_REV n (x DIV 2) (2 * y + SBIT (ODD x) 0))``,
-   rec_axiom = prim_recTheory.num_Axiom};
+   Prim_rec.new_recursive_definition
+     {name = "BIT_REV_def",
+      def = ``(BIT_REV 0 x y = y) /\
+              (BIT_REV (SUC n) x y =
+               BIT_REV n (x DIV 2) (2 * y + SBIT (ODD x) 0))``,
+      rec_axiom = prim_recTheory.num_Axiom}
 
-val BIT_R = ``\(x,y). (x DIV 2, 2 * y + SBIT (BIT 0 x) 0)``;
+val BIT_R = ``\(x,y). (x DIV 2, 2 * y + SBIT (BIT 0 x) 0)``
 
-val BIT_R_FUNPOW = prove(
-  `!n x y. FUNPOW ^BIT_R (SUC n) (x,y) =
-   (x DIV 2 ** (SUC n), 2 * (SND (FUNPOW ^BIT_R n (x, y))) + SBIT (BIT n x) 0)`,
-  Induct >- SIMP_TAC arith_ss [FUNPOW]
-    \\ `!x n. BIT 0 (x DIV 2 ** n) = BIT n x`
-      by SIMP_TAC std_ss [BIT_def,BITS_THM,BITS_COMP_THM2,DIV_1,SUC_SUB]
-    \\ ASM_SIMP_TAC std_ss [FUNPOW_SUC,DIV_DIV_DIV_MULT,ZERO_LT_TWOEXP,
-           (GSYM o ONCE_REWRITE_RULE [MULT_COMM]) EXP]);
+val BIT_R_FUNPOW = Q.prove(
+   `!n x y.
+      FUNPOW ^BIT_R (SUC n) (x,y) =
+      (x DIV 2 ** (SUC n),
+       2 * (SND (FUNPOW ^BIT_R n (x, y))) + SBIT (BIT n x) 0)`,
+   Induct
+   >- SIMP_TAC arith_ss [FUNPOW]
+   \\ `!x n. BIT 0 (x DIV 2 ** n) = BIT n x`
+   by SIMP_TAC std_ss [BIT_def, BITS_THM, BITS_COMP_THM2, DIV_1, SUC_SUB]
+   \\ ASM_SIMP_TAC std_ss [FUNPOW_SUC, DIV_DIV_DIV_MULT, ZERO_LT_TWOEXP,
+                           (GSYM o ONCE_REWRITE_RULE [MULT_COMM]) EXP])
 
-val BIT_R_BIT_REV = prove(
-  `!n a y. SND (FUNPOW ^BIT_R n (a, y)) = BIT_REV n a y`,
-  Induct >- SIMP_TAC std_ss [FUNPOW,BIT_REV_def]
-    \\ ASM_SIMP_TAC std_ss [FUNPOW,BIT_REV_def,LSB_def,GSYM LSB_ODD]);
+val BIT_R_BIT_REV = Q.prove(
+   `!n a y. SND (FUNPOW ^BIT_R n (a, y)) = BIT_REV n a y`,
+   Induct
+   >- SIMP_TAC std_ss [FUNPOW, BIT_REV_def]
+   \\ ASM_SIMP_TAC std_ss [FUNPOW, BIT_REV_def, GSYM BIT0_ODD])
 
-val BIT_REVERSE_REV = prove(
-  `!m n. BIT_REVERSE m n = SND (FUNPOW ^BIT_R m (n, 0))`,
-  Induct >- SIMP_TAC std_ss [BIT_REVERSE_def,FUNPOW]
-    \\ ASM_SIMP_TAC arith_ss [BIT_REVERSE_def,BIT_R_FUNPOW]);
+val BIT_REVERSE_REV = Q.prove(
+   `!m n. BIT_REVERSE m n = SND (FUNPOW ^BIT_R m (n, 0))`,
+   Induct
+   >- SIMP_TAC std_ss [BIT_REVERSE_def, FUNPOW]
+   \\ ASM_SIMP_TAC arith_ss [BIT_REVERSE_def, BIT_R_FUNPOW])
 
 val BIT_REVERSE_EVAL = save_thm("BIT_REVERSE_EVAL",
-  REWRITE_RULE [BIT_R_BIT_REV] BIT_REVERSE_REV);
+   REWRITE_RULE [BIT_R_BIT_REV] BIT_REVERSE_REV)
 
 (* ------------------------------------------------------------------------- *)
 
 val BIT_MODF_def =
   Prim_rec.new_recursive_definition
-  {name = "BIT_MODF_def",
-   def = ``(BIT_MODF 0 f x b e y = y)
-        /\ (BIT_MODF (SUC n) f x b e y =
-              BIT_MODF n f (x DIV 2) (b + 1) (2 * e)
-                (if f b (ODD x) then e + y else y))``,
-   rec_axiom = prim_recTheory.num_Axiom};
+     {name = "BIT_MODF_def",
+      def = ``(BIT_MODF 0 f x b e y = y) /\
+              (BIT_MODF (SUC n) f x b e y =
+                 BIT_MODF n f (x DIV 2) (b + 1) (2 * e)
+                   (if f b (ODD x) then e + y else y))``,
+      rec_axiom = prim_recTheory.num_Axiom}
 
 val BIT_M =
-  ``\(y,f,x,b,e).
-       (if f b (BIT 0 x) then e + y else y, f, x DIV 2, b + 1, 2 * e)``;
+   ``\(y,f,x,b,e).
+        (if f b (BIT 0 x) then e + y else y, f, x DIV 2, b + 1, 2 * e)``
 
-val BIT_M_FUNPOW = prove(
-  `!n f x b e y. FUNPOW ^BIT_M (SUC n) (y,f,x,b,e) =
-       (if f (b + n) (BIT n x)
-        then 2 ** n * e + FST (FUNPOW ^BIT_M n (y,f,x,b,e))
-        else FST (FUNPOW ^BIT_M n (y,f,x,b,e)),
-        f, x DIV 2 ** (SUC n), b + SUC n, 2 ** SUC n * e)`,
-  Induct >- SIMP_TAC arith_ss [FUNPOW]
-    \\ `!x n. BIT 0 (x DIV 2 ** n) = BIT n x`
-      by SIMP_TAC std_ss [BIT_def,BITS_THM,BITS_COMP_THM2,DIV_1,SUC_SUB]
-    \\ ASM_SIMP_TAC arith_ss [FUNPOW_SUC,DIV_DIV_DIV_MULT,ZERO_LT_TWOEXP,
-           (GSYM o ONCE_REWRITE_RULE [MULT_COMM]) EXP]
-    \\ SIMP_TAC (std_ss++numSimps.ARITH_AC_ss) [EXP]);
+val BIT_M_FUNPOW = Q.prove(
+   `!n f x b e y. FUNPOW ^BIT_M (SUC n) (y,f,x,b,e) =
+        (if f (b + n) (BIT n x)
+            then 2 ** n * e + FST (FUNPOW ^BIT_M n (y,f,x,b,e))
+         else FST (FUNPOW ^BIT_M n (y,f,x,b,e)),
+         f, x DIV 2 ** (SUC n), b + SUC n, 2 ** SUC n * e)`,
+   Induct
+   >- SIMP_TAC arith_ss [FUNPOW]
+   \\ `!x n. BIT 0 (x DIV 2 ** n) = BIT n x`
+   by SIMP_TAC std_ss [BIT_def, BITS_THM, BITS_COMP_THM2, DIV_1, SUC_SUB]
+   \\ ASM_SIMP_TAC arith_ss
+        [FUNPOW_SUC, DIV_DIV_DIV_MULT, ZERO_LT_TWOEXP,
+         (GSYM o ONCE_REWRITE_RULE [MULT_COMM]) EXP]
+   \\ SIMP_TAC (std_ss++numSimps.ARITH_AC_ss) [EXP])
 
-val BIT_M_BIT_MODF = prove(
-  `!n f x b e y. FST (FUNPOW ^BIT_M n (y,f,x,b,e)) = BIT_MODF n f x b e y`,
-  Induct >- SIMP_TAC std_ss [FUNPOW,BIT_MODF_def]
-    \\ ASM_SIMP_TAC std_ss [FUNPOW,BIT_MODF_def,LSB_def,GSYM LSB_ODD]);
+val BIT_M_BIT_MODF = Q.prove(
+   `!n f x b e y. FST (FUNPOW ^BIT_M n (y,f,x,b,e)) = BIT_MODF n f x b e y`,
+   Induct
+   >- SIMP_TAC std_ss [FUNPOW, BIT_MODF_def]
+   \\ ASM_SIMP_TAC std_ss [FUNPOW, BIT_MODF_def, GSYM BIT0_ODD])
 
-val BIT_MODIFY_MODF = prove(
-  `!m f n. BIT_MODIFY m f n = FST (FUNPOW ^BIT_M m (0,f,n,0,1))`,
-  Induct >- SIMP_TAC std_ss [BIT_MODIFY_def,FUNPOW]
-    \\ RW_TAC arith_ss [SBIT_def,BIT_MODIFY_def,BIT_M_FUNPOW]);
+val BIT_MODIFY_MODF = Q.prove(
+   `!m f n. BIT_MODIFY m f n = FST (FUNPOW ^BIT_M m (0,f,n,0,1))`,
+   Induct
+   >- SIMP_TAC std_ss [BIT_MODIFY_def, FUNPOW]
+   \\ RW_TAC arith_ss [SBIT_def, BIT_MODIFY_def, BIT_M_FUNPOW])
 
 val BIT_MODIFY_EVAL = save_thm("BIT_MODIFY_EVAL",
-  REWRITE_RULE [BIT_M_BIT_MODF] BIT_MODIFY_MODF);
+   REWRITE_RULE [BIT_M_BIT_MODF] BIT_MODIFY_MODF)
 
 (* ------------------------------------------------------------------------- *)
 
-val SUC_RULE = CONV_RULE numLib.SUC_TO_NUMERAL_DEFN_CONV;
+val SUC_RULE = CONV_RULE numLib.SUC_TO_NUMERAL_DEFN_CONV
 
 val iBITWISE_def =
-  Definition.new_definition("iBITWISE_def", ``iBITWISE = BITWISE``);
+   Definition.new_definition("iBITWISE_def", ``iBITWISE = BITWISE``)
 
-val SIMP_BIT1 = (GSYM o SIMP_RULE arith_ss []) BIT1;
+val SIMP_BIT1 = (GSYM o SIMP_RULE arith_ss []) BIT1
 
-val iBITWISE = prove(
-  `(!opr a b. iBITWISE 0 opr a b = ZERO) /\
-   (!x opr a b.
-     iBITWISE (SUC x) opr a b =
-       let w = iBITWISE x opr (DIV2 a) (DIV2 b) in
-       if opr (ODD a) (ODD b) then BIT1 w else numeral$iDUB w)`,
-  RW_TAC arith_ss [iBITWISE_def,iDUB,SIMP_BIT1,SBIT_def,EXP,
-                   LSB_ODD,GSYM DIV2_def,BITWISE_EVAL,LET_THM]
-    \\ REWRITE_TAC [BITWISE_def,ALT_ZERO]);
+val iBITWISE = Q.prove(
+   `(!opr a b. iBITWISE 0 opr a b = ZERO) /\
+    (!x opr a b.
+      iBITWISE (SUC x) opr a b =
+        let w = iBITWISE x opr (DIV2 a) (DIV2 b) in
+        if opr (ODD a) (ODD b) then BIT1 w else numeral$iDUB w)`,
+   RW_TAC arith_ss [iBITWISE_def, iDUB, SIMP_BIT1, SBIT_def, EXP,
+                    BIT0_ODD, GSYM DIV2_def, BITWISE_EVAL, LET_THM]
+   \\ REWRITE_TAC [BITWISE_def, ALT_ZERO])
 
-val iBITWISE = save_thm("iBITWISE", SUC_RULE iBITWISE);
+val iBITWISE = save_thm("iBITWISE", SUC_RULE iBITWISE)
 
-val NUMERAL_BITWISE = store_thm("NUMERAL_BITWISE",
-  `(!x f a. BITWISE x f 0 0 = NUMERAL (iBITWISE x f 0 0)) /\
-   (!x f a. BITWISE x f (NUMERAL a) 0 =
-              NUMERAL (iBITWISE x f (NUMERAL a) 0)) /\
-   (!x f b. BITWISE x f 0 (NUMERAL b) =
-              NUMERAL (iBITWISE x f 0 (NUMERAL b))) /\
-    !x f a b. BITWISE x f (NUMERAL a) (NUMERAL b) =
-                 NUMERAL (iBITWISE x f (NUMERAL a) (NUMERAL b))`,
-  REWRITE_TAC [iBITWISE_def,NUMERAL_DEF]);
+val NUMERAL_BITWISE = Q.store_thm("NUMERAL_BITWISE",
+   `(!x f a. BITWISE x f 0 0 = NUMERAL (iBITWISE x f 0 0)) /\
+    (!x f a. BITWISE x f (NUMERAL a) 0 =
+             NUMERAL (iBITWISE x f (NUMERAL a) 0)) /\
+    (!x f b. BITWISE x f 0 (NUMERAL b) =
+             NUMERAL (iBITWISE x f 0 (NUMERAL b))) /\
+     !x f a b. BITWISE x f (NUMERAL a) (NUMERAL b) =
+               NUMERAL (iBITWISE x f (NUMERAL a) (NUMERAL b))`,
+   REWRITE_TAC [iBITWISE_def, NUMERAL_DEF])
 
-val NUMERAL_BIT_REV = prove(
-  `(!x y. BIT_REV 0 x y = y) /\
-   (!n y. BIT_REV (SUC n) 0 y = BIT_REV n 0 (numeral$iDUB y)) /\
-   (!n x y. BIT_REV (SUC n) (NUMERAL x) y =
-      BIT_REV n (DIV2 (NUMERAL x)) (if ODD x then BIT1 y
-                                    else numeral$iDUB y))`,
-  RW_TAC bool_ss [BIT_REV_def,SBIT_def,NUMERAL_DEF,DIV2_def,
-           ADD,ADD_0,BIT2,BIT1,iDUB,ALT_ZERO]
-    \\ FULL_SIMP_TAC arith_ss []);
+val NUMERAL_BIT_REV = Q.prove(
+   `(!x y. BIT_REV 0 x y = y) /\
+    (!n y. BIT_REV (SUC n) 0 y = BIT_REV n 0 (numeral$iDUB y)) /\
+    (!n x y. BIT_REV (SUC n) (NUMERAL x) y =
+             BIT_REV n (DIV2 (NUMERAL x))
+                (if ODD x then BIT1 y else numeral$iDUB y))`,
+   RW_TAC bool_ss [BIT_REV_def, SBIT_def, NUMERAL_DEF, DIV2_def,
+                   ADD, ADD_0, BIT2, BIT1, iDUB, ALT_ZERO]
+   \\ FULL_SIMP_TAC arith_ss [])
 
-val NUMERAL_BIT_REV = save_thm("NUMERAL_BIT_REV", SUC_RULE NUMERAL_BIT_REV);
+val NUMERAL_BIT_REV = save_thm("NUMERAL_BIT_REV", SUC_RULE NUMERAL_BIT_REV)
 
-val NUMERAL_BIT_REVERSE = store_thm("NUMERAL_BIT_REVERSE",
-  `(!m. BIT_REVERSE (NUMERAL m) 0 = NUMERAL (BIT_REV (NUMERAL m) 0 ZERO)) /\
-    !n m. BIT_REVERSE (NUMERAL m) (NUMERAL n) =
-       NUMERAL (BIT_REV (NUMERAL m) (NUMERAL n) ZERO)`,
-  SIMP_TAC bool_ss [NUMERAL_DEF,ALT_ZERO,BIT_REVERSE_EVAL]);
+val NUMERAL_BIT_REVERSE = Q.store_thm("NUMERAL_BIT_REVERSE",
+   `(!m. BIT_REVERSE (NUMERAL m) 0 = NUMERAL (BIT_REV (NUMERAL m) 0 ZERO)) /\
+     !n m. BIT_REVERSE (NUMERAL m) (NUMERAL n) =
+           NUMERAL (BIT_REV (NUMERAL m) (NUMERAL n) ZERO)`,
+   SIMP_TAC bool_ss [NUMERAL_DEF, ALT_ZERO, BIT_REVERSE_EVAL])
 
-val NUMERAL_BIT_MODF = prove(
-  `(!f x b e y. BIT_MODF 0 f x b e y = y) /\
-   (!n f b e y. BIT_MODF (SUC n) f 0 b (NUMERAL e) y =
-      BIT_MODF n f 0 (b + 1) (NUMERAL (numeral$iDUB e))
-              (if f b F then (NUMERAL e) + y else y)) /\
-   (!n f x b e y. BIT_MODF (SUC n) f (NUMERAL x) b (NUMERAL e) y =
-      BIT_MODF n f (DIV2 (NUMERAL x)) (b + 1) (NUMERAL (numeral$iDUB e))
-              (if f b (ODD x) then (NUMERAL e) + y else y))`,
-  RW_TAC bool_ss [BIT_MODF_def,SBIT_def,NUMERAL_DEF,DIV2_def,
-           ADD,ADD_0,BIT2,BIT1,iDUB,ALT_ZERO]
-    \\ FULL_SIMP_TAC arith_ss []);
+val NUMERAL_BIT_MODF = Q.prove(
+   `(!f x b e y. BIT_MODF 0 f x b e y = y) /\
+    (!n f b e y.
+       BIT_MODF (SUC n) f 0 b (NUMERAL e) y =
+       BIT_MODF n f 0 (b + 1) (NUMERAL (numeral$iDUB e))
+          (if f b F then (NUMERAL e) + y else y)) /\
+    (!n f x b e y.
+       BIT_MODF (SUC n) f (NUMERAL x) b (NUMERAL e) y =
+       BIT_MODF n f (DIV2 (NUMERAL x)) (b + 1) (NUMERAL (numeral$iDUB e))
+          (if f b (ODD x) then (NUMERAL e) + y else y))`,
+   RW_TAC bool_ss [BIT_MODF_def, SBIT_def, NUMERAL_DEF, DIV2_def,
+                   ADD, ADD_0, BIT2, BIT1, iDUB, ALT_ZERO]
+   \\ FULL_SIMP_TAC arith_ss [])
 
-val NUMERAL_BIT_MODF = save_thm("NUMERAL_BIT_MODF", SUC_RULE NUMERAL_BIT_MODF);
+val NUMERAL_BIT_MODF = save_thm("NUMERAL_BIT_MODF", SUC_RULE NUMERAL_BIT_MODF)
 
-val NUMERAL_BIT_MODIFY = store_thm("NUMERAL_BIT_MODIFY",
+val NUMERAL_BIT_MODIFY = Q.store_thm("NUMERAL_BIT_MODIFY",
   `(!m f. BIT_MODIFY (NUMERAL m) f 0 = BIT_MODF (NUMERAL m) f 0 0 1 0) /\
     !m f n. BIT_MODIFY (NUMERAL m) f (NUMERAL n) =
-       BIT_MODF (NUMERAL m) f (NUMERAL n) 0 1 0`,
-  SIMP_TAC bool_ss [NUMERAL_DEF,ALT_ZERO,BIT_MODIFY_EVAL]);
+            BIT_MODF (NUMERAL m) f (NUMERAL n) 0 1 0`,
+  SIMP_TAC bool_ss [NUMERAL_DEF, ALT_ZERO, BIT_MODIFY_EVAL])
 
 (* ------------------------------------------------------------------------- *)
 
-val iSUC_def =
-  Definition.new_definition
-    ("iSUC",``iSUC = SUC``);
+val iSUC_def = Definition.new_definition ("iSUC",``iSUC = SUC``)
 
-val iDIV2_def =
-  Definition.new_definition
-    ("iDIV2",``iDIV2 = DIV2``);
+val iDIV2_def = Definition.new_definition ("iDIV2",``iDIV2 = DIV2``)
 
 val SFUNPOW_def =
   Prim_rec.new_recursive_definition
-  {name = "SFUNPOW_def",
-   def = ``(SFUNPOW f 0 x = x)
-        /\ (SFUNPOW f (SUC n) x = if x = 0n then 0n else SFUNPOW f n (f x))``,
-   rec_axiom = prim_recTheory.num_Axiom};
+    {name = "SFUNPOW_def",
+     def = ``(SFUNPOW f 0 x = x) /\
+             (SFUNPOW f (SUC n) x = if x = 0n then 0n else SFUNPOW f n (f x))``,
+     rec_axiom = prim_recTheory.num_Axiom}
 
 val FDUB_def =
    Prim_rec.new_recursive_definition
-   {name = "FDUB_def",
-    def = ``(FDUB f 0 = 0n)
-         /\ (FDUB f (SUC n) = f (f (SUC n)))``,
-   rec_axiom = prim_recTheory.num_Axiom};
+      {name = "FDUB_def",
+       def = ``(FDUB f 0 = 0n) /\
+               (FDUB f (SUC n) = f (f (SUC n)))``,
+      rec_axiom = prim_recTheory.num_Axiom}
 
-val FDUB_lem = prove(
-  `!f. (f 0 = 0n) ==> (FDUB f = (\x.f (f x)))`,
-  REWRITE_TAC [FUN_EQ_THM] \\ GEN_TAC \\
-  DISCH_TAC \\ BETA_TAC \\ Cases \\
-  ASM_REWRITE_TAC [FDUB_def]);
+val FDUB_lem = Q.prove(
+   `!f. (f 0 = 0n) ==> (FDUB f = (\x.f (f x)))`,
+   REWRITE_TAC [FUN_EQ_THM]
+   \\ GEN_TAC
+   \\ DISCH_TAC
+   \\ BETA_TAC
+   \\ Cases
+   \\ ASM_REWRITE_TAC [FDUB_def])
 
-val SFUNPOW_strict = prove(
+val SFUNPOW_strict = Q.prove(
    `!n f x. SFUNPOW f n 0 = 0`,
-   Cases \\ REWRITE_TAC [SFUNPOW_def]);
+   Cases \\ REWRITE_TAC [SFUNPOW_def])
 
-val SFUNPOW_BIT1_lem = prove(
-   `!n f x. (f 0 = 0) ==>
+val SFUNPOW_BIT1_lem = Q.prove(
+   `!n f x.
+      (f 0 = 0) ==>
       (SFUNPOW f (NUMERAL (BIT1 n)) x = SFUNPOW (FDUB f) n (f x))`,
-   REWRITE_TAC [NUMERAL_DEF,BIT1,ADD_CLAUSES]
-   \\ Induct \\ REPEAT STRIP_TAC \\ REWRITE_TAC [NUMERAL_DEF,BIT1,ADD_CLAUSES]
+   REWRITE_TAC [NUMERAL_DEF, BIT1, ADD_CLAUSES]
+   \\ Induct
+   \\ REPEAT STRIP_TAC
+   \\ REWRITE_TAC [NUMERAL_DEF, BIT1, ADD_CLAUSES]
    >- (IMP_RES_TAC FDUB_lem \\ ASM_REWRITE_TAC [SFUNPOW_def] \\ PROVE_TAC [])
-   \\ ONCE_REWRITE_TAC [SFUNPOW_def] \\ ONCE_REWRITE_TAC [SFUNPOW_def]
-   \\ RES_TAC \\ RW_TAC std_ss [] \\ IMP_RES_TAC FDUB_lem \\ PROVE_TAC []);
+   \\ ONCE_REWRITE_TAC [SFUNPOW_def]
+   \\ ONCE_REWRITE_TAC [SFUNPOW_def]
+   \\ RES_TAC
+   \\ RW_TAC std_ss []
+   \\ IMP_RES_TAC FDUB_lem
+   \\ PROVE_TAC [])
 
-val SFUNPOW_BIT2_lem = prove(
-  `!n f x. (f 0 = 0) ==>
-     (SFUNPOW f (NUMERAL (BIT2 n)) x = SFUNPOW (FDUB f) n (f (f x)))`,
-  `!n. NUMERAL (BIT2 n) = SUC (NUMERAL (BIT1 n))` by
-             REWRITE_TAC [NUMERAL_DEF,BIT1,BIT2,ADD_CLAUSES] \\
-  REPEAT STRIP_TAC \\ IMP_RES_TAC SFUNPOW_BIT1_lem \\
-  ASM_REWRITE_TAC [SFUNPOW_def] \\ RW_TAC std_ss [SFUNPOW_strict]);
+val SFUNPOW_BIT2_lem = Q.prove(
+   `!n f x.
+      (f 0 = 0) ==>
+      (SFUNPOW f (NUMERAL (BIT2 n)) x = SFUNPOW (FDUB f) n (f (f x)))`,
+   `!n. NUMERAL (BIT2 n) = SUC (NUMERAL (BIT1 n))`
+   by REWRITE_TAC [NUMERAL_DEF, BIT1, BIT2, ADD_CLAUSES]
+   \\ REPEAT STRIP_TAC
+   \\ IMP_RES_TAC SFUNPOW_BIT1_lem
+   \\ ASM_REWRITE_TAC [SFUNPOW_def]
+   \\ RW_TAC std_ss [SFUNPOW_strict])
 
-val NUMERAL_SFUNPOW = prove(
+val NUMERAL_SFUNPOW = Q.prove(
   `!f. (f 0 = 0) ==>
-      (!x. SFUNPOW f 0 x = x)
-   /\ (!y. SFUNPOW f y 0 = 0)
-   /\ (!n x. SFUNPOW f (NUMERAL (BIT1 n)) x = SFUNPOW (FDUB f) (NUMERAL n) (f x))
-   /\ (!n x. SFUNPOW f (NUMERAL (BIT2 n)) x = SFUNPOW (FDUB f) (NUMERAL n) (f (f x)))`,
-  REPEAT STRIP_TAC \\
-  MAP_EVERY IMP_RES_TAC [SFUNPOW_BIT1_lem,SFUNPOW_BIT2_lem] \\
-  ASM_REWRITE_TAC [SFUNPOW_strict,SFUNPOW_def,NUMERAL_DEF]);
+       (!x. SFUNPOW f 0 x = x) /\
+       (!y. SFUNPOW f y 0 = 0) /\
+       (!n x. SFUNPOW f (NUMERAL (BIT1 n)) x =
+              SFUNPOW (FDUB f) (NUMERAL n) (f x)) /\
+       (!n x. SFUNPOW f (NUMERAL (BIT2 n)) x =
+              SFUNPOW (FDUB f) (NUMERAL n) (f (f x)))`,
+   REPEAT STRIP_TAC
+   \\ MAP_EVERY IMP_RES_TAC [SFUNPOW_BIT1_lem, SFUNPOW_BIT2_lem]
+   \\ ASM_REWRITE_TAC [SFUNPOW_strict, SFUNPOW_def, NUMERAL_DEF])
 
-val NUMERAL_TIMES_2EXP = store_thm("NUMERAL_TIMES_2EXP",
-  `(!n. TIMES_2EXP n 0 = 0) /\
-   (!n x. TIMES_2EXP n (NUMERAL x) = NUMERAL (SFUNPOW numeral$iDUB n x))`,
-  CONJ_TAC \\ REWRITE_TAC [TIMES_2EXP_def,MULT_CLAUSES] \\ Induct \\
-  REWRITE_TAC [EXP,SFUNPOW_def,MULT_CLAUSES,MULT_ASSOC] \\
-  POP_ASSUM (ASSUME_TAC o GSYM) \\ RW_TAC std_ss [] \\
-  ASM_REWRITE_TAC [NUMERAL_DEF,BIT1,BIT2,iDUB,ALT_ZERO,ADD_CLAUSES] \\
-  RW_TAC arith_ss []);
+val NUMERAL_TIMES_2EXP = Q.store_thm("NUMERAL_TIMES_2EXP",
+   `(!n. TIMES_2EXP n 0 = 0) /\
+    (!n x. TIMES_2EXP n (NUMERAL x) = NUMERAL (SFUNPOW numeral$iDUB n x))`,
+   CONJ_TAC
+   \\ REWRITE_TAC [TIMES_2EXP_def, MULT_CLAUSES]
+   \\ Induct
+   \\ REWRITE_TAC [EXP, SFUNPOW_def, MULT_CLAUSES, MULT_ASSOC]
+   \\ POP_ASSUM (ASSUME_TAC o GSYM)
+   \\ RW_TAC std_ss []
+   \\ ASM_REWRITE_TAC [NUMERAL_DEF, BIT1, BIT2, iDUB, ALT_ZERO, ADD_CLAUSES]
+   \\ RW_TAC arith_ss [])
 
-val NUMERAL_iDIV2 = store_thm("NUMERAL_iDIV2",
-  `(iDIV2 ZERO = ZERO) /\ (iDIV2 (iSUC ZERO) = ZERO) /\
-   (iDIV2 (BIT1 n) = n) /\ (iDIV2 (iSUC (BIT1 n)) = iSUC n) /\
-   (iDIV2 (BIT2 n) = iSUC n) /\ (iDIV2 (iSUC (BIT2 n)) = iSUC n) /\
-   (NUMERAL (iSUC n) = NUMERAL (SUC n))`,
-   REWRITE_TAC [ALT_ZERO,BIT1,BIT2,iDIV2_def,iSUC_def,ADD_CLAUSES] \\
-   REWRITE_TAC [DIV2_def,GSYM TIMES2] \\
-   `0 < 2 /\ 1 < 2` by DECIDE_TAC \\
-   MAP_EVERY IMP_RES_TAC [ZERO_DIV,ADD_DIV_RWT,DIV_LESS,
-        LESS_DIV_EQ_ZERO,ONCE_REWRITE_RULE [MULT_COMM] MULT_DIV] \\
-   RULE_ASSUM_TAC (REWRITE_RULE [GSYM EVEN_MOD2]) \\
-   RW_TAC arith_ss [ADD1,EVEN_DOUBLE]);
+val NUMERAL_iDIV2 = Q.store_thm("NUMERAL_iDIV2",
+   `(iDIV2 ZERO = ZERO) /\
+    (iDIV2 (iSUC ZERO) = ZERO) /\
+    (iDIV2 (BIT1 n) = n) /\
+    (iDIV2 (iSUC (BIT1 n)) = iSUC n) /\
+    (iDIV2 (BIT2 n) = iSUC n) /\
+    (iDIV2 (iSUC (BIT2 n)) = iSUC n) /\
+    (NUMERAL (iSUC n) = NUMERAL (SUC n))`,
+   REWRITE_TAC [ALT_ZERO, BIT1, BIT2, iDIV2_def, iSUC_def, ADD_CLAUSES]
+   \\ REWRITE_TAC [DIV2_def, GSYM TIMES2]
+   \\ `0 < 2 /\ 1 < 2` by DECIDE_TAC
+   \\ MAP_EVERY IMP_RES_TAC
+        [ZERO_DIV, ADD_DIV_RWT, DIV_LESS,
+         LESS_DIV_EQ_ZERO, ONCE_REWRITE_RULE [MULT_COMM] MULT_DIV]
+   \\ RULE_ASSUM_TAC (REWRITE_RULE [GSYM EVEN_MOD2])
+   \\ RW_TAC arith_ss [ADD1, EVEN_DOUBLE])
 
-val NUMERAL_DIV_2EXP = store_thm("NUMERAL_DIV_2EXP",
-  `(!n. DIV_2EXP n 0 = 0) /\
-   (!n x. DIV_2EXP n (NUMERAL x) = NUMERAL (SFUNPOW iDIV2 n x))`,
-  CONJ_TAC \\ REWRITE_TAC [DIV_2EXP_def]
-  >- (STRIP_TAC \\ MATCH_MP_TAC ZERO_DIV \\ RW_TAC std_ss [ZERO_LT_TWOEXP])
-  \\ Induct \\ REWRITE_TAC [EXP,SFUNPOW_def,DIV_1]
-  \\ `!x. NUMERAL x DIV 2 = NUMERAL (x DIV 2)` by REWRITE_TAC [NUMERAL_DEF]
-  \\ RW_TAC arith_ss
-      [ZERO_LT_TWOEXP,GSYM DIV_DIV_DIV_MULT,SFUNPOW_strict,iDIV2_def,DIV2_def]);
+val NUMERAL_DIV_2EXP = Q.store_thm("NUMERAL_DIV_2EXP",
+   `(!n. DIV_2EXP n 0 = 0) /\
+    (!n x. DIV_2EXP n (NUMERAL x) = NUMERAL (SFUNPOW iDIV2 n x))`,
+   CONJ_TAC
+   \\ REWRITE_TAC [DIV_2EXP_def]
+   >- (STRIP_TAC \\ MATCH_MP_TAC ZERO_DIV \\ RW_TAC std_ss [ZERO_LT_TWOEXP])
+   \\ Induct
+   \\ REWRITE_TAC [EXP, SFUNPOW_def, DIV_1]
+   \\ `!x. NUMERAL x DIV 2 = NUMERAL (x DIV 2)` by REWRITE_TAC [NUMERAL_DEF]
+   \\ RW_TAC arith_ss
+         [ZERO_LT_TWOEXP, GSYM DIV_DIV_DIV_MULT, SFUNPOW_strict, iDIV2_def,
+          DIV2_def])
 
-val NUMERAL_SFUNPOW_iDIV2 =
-  save_thm("NUMERAL_SFUNPOW_iDIV2",
-    MATCH_MP (SPEC_ALL NUMERAL_SFUNPOW)
-    (prove(
-       `iDIV2 0 = 0`,RW_TAC arith_ss [iDIV2_def,DIV2_def])));
+val NUMERAL_SFUNPOW_iDIV2 = save_thm("NUMERAL_SFUNPOW_iDIV2",
+   MATCH_MP (SPEC_ALL NUMERAL_SFUNPOW)
+      (Q.prove(`iDIV2 0 = 0`, RW_TAC arith_ss [iDIV2_def, DIV2_def])))
 
-val NUMERAL_SFUNPOW_iDUB =
-  save_thm("NUMERAL_SFUNPOW_iDUB",
-    MATCH_MP (SPEC_ALL NUMERAL_SFUNPOW)
-    (prove(
-       `numeral$iDUB 0 = 0`,RW_TAC arith_ss [iDUB])));
+val NUMERAL_SFUNPOW_iDUB = save_thm("NUMERAL_SFUNPOW_iDUB",
+   MATCH_MP (SPEC_ALL NUMERAL_SFUNPOW)
+      (Q.prove(`numeral$iDUB 0 = 0`, RW_TAC arith_ss [iDUB])))
 
-val NUMERAL_SFUNPOW_FDUB =
-  save_thm("NUMERAL_SFUNPOW_FDUB",
-    GEN_ALL (MATCH_MP
-      (SPEC_ALL NUMERAL_SFUNPOW)
-      (SPEC_ALL (CONJUNCT1 FDUB_def))));
+val NUMERAL_SFUNPOW_FDUB = save_thm("NUMERAL_SFUNPOW_FDUB",
+   GEN_ALL (MATCH_MP (SPEC_ALL NUMERAL_SFUNPOW)
+                     (SPEC_ALL (CONJUNCT1 FDUB_def))))
 
-val FDUB_iDIV2 = store_thm("FDUB_iDIV2",
-  `!x. FDUB iDIV2 x = iDIV2 (iDIV2 x)`,
-  Cases \\ RW_TAC arith_ss [FDUB_def,iDIV2_def,DIV2_def]);
+val FDUB_iDIV2 = Q.store_thm("FDUB_iDIV2",
+   `!x. FDUB iDIV2 x = iDIV2 (iDIV2 x)`,
+   Cases \\ RW_TAC arith_ss [FDUB_def, iDIV2_def, DIV2_def])
 
-val FDUB_iDUB = store_thm("FDUB_iDUB",
-  `!x. FDUB numeral$iDUB x = numeral$iDUB (numeral$iDUB x)`,
-  Cases \\ RW_TAC arith_ss [FDUB_def,iDUB]);
+val FDUB_iDUB = Q.store_thm("FDUB_iDUB",
+   `!x. FDUB numeral$iDUB x = numeral$iDUB (numeral$iDUB x)`,
+   Cases \\ RW_TAC arith_ss [FDUB_def, iDUB])
 
-val FDUB_FDUB = store_thm("FDUB_FDUB",
-  `   (FDUB (FDUB f) ZERO = ZERO)
-   /\ (!x. FDUB (FDUB f) (iSUC x) = FDUB f (FDUB f (iSUC x)))
-   /\ (!x. FDUB (FDUB f) (BIT1 x) = FDUB f (FDUB f (BIT1 x)))
-   /\ (!x. FDUB (FDUB f) (BIT2 x) = FDUB f (FDUB f (BIT2 x)))`,
-  REWRITE_TAC [BIT1,BIT2,iSUC_def,FDUB_def,ALT_ZERO,ADD_CLAUSES]);
+val FDUB_FDUB = Q.store_thm("FDUB_FDUB",
+   `(FDUB (FDUB f) ZERO = ZERO) /\
+    (!x. FDUB (FDUB f) (iSUC x) = FDUB f (FDUB f (iSUC x))) /\
+    (!x. FDUB (FDUB f) (BIT1 x) = FDUB f (FDUB f (BIT1 x))) /\
+    (!x. FDUB (FDUB f) (BIT2 x) = FDUB f (FDUB f (BIT2 x)))`,
+   REWRITE_TAC [BIT1, BIT2, iSUC_def, FDUB_def, ALT_ZERO, ADD_CLAUSES])
 
 (* ------------------------------------------------------------------------- *)
 
-val LOG_compute = store_thm("LOG_compute",
-  `!m n. LOG m n =
-         if m < 2 \/ (n = 0) then
-           FAIL LOG ^(mk_var("base < 2 or n = 0", bool)) m n
-         else
-           if n < m then
-             0
-           else
-             SUC (LOG m (n DIV m))`,
-  SRW_TAC [ARITH_ss] [logrootTheory.LOG_RWT, combinTheory.FAIL_THM]);
+val LOG_compute = Q.store_thm("LOG_compute",
+   `!m n. LOG m n =
+          if m < 2 \/ (n = 0) then
+            FAIL LOG ^(mk_var("base < 2 or n = 0", bool)) m n
+          else
+            if n < m then
+              0
+            else
+              SUC (LOG m (n DIV m))`,
+   SRW_TAC [ARITH_ss] [logrootTheory.LOG_RWT, combinTheory.FAIL_THM])
 
 val iLOG2_def =
- Definition.new_definition("iLOG2_def", ``iLOG2 n = LOG2 (n + 1)``);
+   Definition.new_definition("iLOG2_def", ``iLOG2 n = LOG2 (n + 1)``)
 
-val LOG2_1 = (SIMP_RULE arith_ss [] o SPECL [`1`,`0`]) LOG2_UNIQUE;
+val LOG2_1 = (SIMP_RULE arith_ss [] o Q.SPECL [`1`,`0`]) LOG2_UNIQUE
 
-val numeral_ilog2 = store_thm("numeral_ilog2",
-  `(iLOG2 ZERO = 0) /\
-   (!n. iLOG2 (BIT1 n) = 1 + iLOG2 n) /\
-   (!n. iLOG2 (BIT2 n) = 1 + iLOG2 n)`,
-  RW_TAC bool_ss [ALT_ZERO,NUMERAL_DEF,BIT1,BIT2,iLOG2_def]
-    \\ SIMP_TAC arith_ss [LOG2_1]
-    >| [
-      MATCH_MP_TAC ((SIMP_RULE arith_ss [] o
-              SPECL [`2 * n + 2`,`LOG2 (n + 1) + 1`]) LOG2_UNIQUE)
-        \\ SIMP_TAC arith_ss [EXP_ADD,LOG2_def]
-        \\ SIMP_TAC arith_ss [GSYM ADD1,EXP,logrootTheory.LOG,
-            DECIDE ``(2 * n + 2 = (n + 1) * 2) /\ (2 * a < 4 * b = a < 2 * b)``]
-        \\ SIMP_TAC arith_ss [GSYM EXP,logrootTheory.LOG],
-      MATCH_MP_TAC ((SIMP_RULE arith_ss [] o
-              SPECL [`2 * n + 3`,`LOG2 (n + 1) + 1`]) LOG2_UNIQUE)
-        \\ SIMP_TAC arith_ss [EXP_ADD,LOG2_def]
-        \\ SIMP_TAC arith_ss [GSYM ADD1,EXP,logrootTheory.LOG,
+val numeral_ilog2 = Q.store_thm("numeral_ilog2",
+   `(iLOG2 ZERO = 0) /\
+    (!n. iLOG2 (BIT1 n) = 1 + iLOG2 n) /\
+    (!n. iLOG2 (BIT2 n) = 1 + iLOG2 n)`,
+   RW_TAC bool_ss [ALT_ZERO, NUMERAL_DEF, BIT1, BIT2, iLOG2_def]
+   \\ SIMP_TAC arith_ss [LOG2_1]
+   >| [
+      MATCH_MP_TAC
+         ((SIMP_RULE arith_ss [] o Q.SPECL [`2 * n + 2`, `LOG2 (n + 1) + 1`])
+             LOG2_UNIQUE)
+      \\ SIMP_TAC arith_ss [EXP_ADD, LOG2_def]
+      \\ SIMP_TAC arith_ss
+            [GSYM ADD1, EXP, logrootTheory.LOG,
+             DECIDE ``(2 * n + 2 = (n + 1) * 2) /\
+                      (2 * a < 4 * b = a < 2 * b)``]
+      \\ SIMP_TAC arith_ss [GSYM EXP, logrootTheory.LOG],
+      MATCH_MP_TAC
+         ((SIMP_RULE arith_ss [] o Q.SPECL [`2 * n + 3`, `LOG2 (n + 1) + 1`])
+             LOG2_UNIQUE)
+      \\ SIMP_TAC arith_ss [EXP_ADD, LOG2_def]
+      \\ SIMP_TAC arith_ss
+            [GSYM ADD1, EXP, logrootTheory.LOG,
              DECIDE ``(2 * n + 3 = 2 * (n + 1) + 1)``,
              DECIDE ``a <= b ==> 2 * a <= SUC (2 * b)``]
-        \\ SIMP_TAC arith_ss [
-             DECIDE ``a < 2 * b ==> SUC (2 * a) < 4 * b``,
-             (Once o GSYM) EXP,logrootTheory.LOG]]);
+      \\ SIMP_TAC arith_ss
+            [DECIDE ``a < 2 * b ==> SUC (2 * a) < 4 * b``,
+             (Once o GSYM) EXP, logrootTheory.LOG]
+   ])
 
-val numeral_log2 = store_thm("numeral_log2",
-  `(!n. LOG2 (NUMERAL (BIT1 n)) = iLOG2 (numeral$iDUB n)) /\
-   (!n. LOG2 (NUMERAL (BIT2 n)) = iLOG2 (BIT1 n))`,
-  RW_TAC bool_ss [ALT_ZERO,NUMERAL_DEF,BIT1,BIT2,iLOG2_def,numeralTheory.iDUB]
-    \\ SIMP_TAC arith_ss []);
+val numeral_log2 = Q.store_thm("numeral_log2",
+   `(!n. LOG2 (NUMERAL (BIT1 n)) = iLOG2 (numeral$iDUB n)) /\
+    (!n. LOG2 (NUMERAL (BIT2 n)) = iLOG2 (BIT1 n))`,
+   RW_TAC bool_ss [ALT_ZERO, NUMERAL_DEF, BIT1, BIT2, iLOG2_def,
+                   numeralTheory.iDUB]
+   \\ SIMP_TAC arith_ss [])
 
 (* ------------------------------------------------------------------------- *)
 
-val MOD_2EXP_EQ = store_thm("MOD_2EXP_EQ",
- `(!a b. MOD_2EXP_EQ 0 a b = T) /\
-  (!n a b. MOD_2EXP_EQ (SUC n) a b =
-     (ODD a = ODD b) /\ MOD_2EXP_EQ n (DIV2 a) (DIV2 b)) /\
-  (!n a. MOD_2EXP_EQ n a a = T)`,
-  SRW_TAC [] [MOD_2EXP_EQ_def, MOD_2EXP_def, GSYM BITS_ZERO3]
-    \\ Cases_on `n`
-    \\ FULL_SIMP_TAC std_ss [GSYM BITS_ZERO3, SYM LSB_ODD, LSB_def,
-         GSYM BIT_BITS_THM, BIT_DIV2, DIV2_def]
-    \\ EQ_TAC \\ RW_TAC arith_ss []
-    \\ Cases_on `x` \\ RW_TAC arith_ss []);
+val MOD_2EXP_EQ = Q.store_thm("MOD_2EXP_EQ",
+   `(!a b. MOD_2EXP_EQ 0 a b = T) /\
+    (!n a b.
+       MOD_2EXP_EQ (SUC n) a b =
+       (ODD a = ODD b) /\ MOD_2EXP_EQ n (DIV2 a) (DIV2 b)) /\
+    (!n a. MOD_2EXP_EQ n a a = T)`,
+   SRW_TAC [] [MOD_2EXP_EQ_def, MOD_2EXP_def, GSYM BITS_ZERO3]
+   \\ Cases_on `n`
+   \\ FULL_SIMP_TAC std_ss [GSYM BITS_ZERO3, GSYM BIT0_ODD,
+                            GSYM BIT_BITS_THM, BIT_DIV2, DIV2_def]
+   \\ EQ_TAC
+   \\ RW_TAC arith_ss []
+   \\ Cases_on `x`
+   \\ RW_TAC arith_ss [])
 
-val lem = prove(
-  `!n. BITS n 0 (2 ** SUC n - 1) = 2 ** SUC n - 1`,
-  STRIP_TAC \\ MATCH_MP_TAC BITS_ZEROL
-    \\ SIMP_TAC std_ss [ZERO_LT_TWOEXP]);
+val lem = Q.prove(
+   `!n. BITS n 0 (2 ** SUC n - 1) = 2 ** SUC n - 1`,
+   STRIP_TAC
+   \\ MATCH_MP_TAC BITS_ZEROL
+   \\ SIMP_TAC std_ss [ZERO_LT_TWOEXP])
 
-val MOD_2EXP_MAX = store_thm("MOD_2EXP_MAX",
- `(!a. MOD_2EXP_MAX 0 a = T) /\
-  (!n a. MOD_2EXP_MAX (SUC n) a = ODD a /\ MOD_2EXP_MAX n (DIV2 a))`,
-  SRW_TAC [] [MOD_2EXP_MAX_def, MOD_2EXP_def, GSYM BITS_ZERO3]
+val MOD_2EXP_MAX = Q.store_thm("MOD_2EXP_MAX",
+   `(!a. MOD_2EXP_MAX 0 a = T) /\
+    (!n a. MOD_2EXP_MAX (SUC n) a = ODD a /\ MOD_2EXP_MAX n (DIV2 a))`,
+    SRW_TAC [] [MOD_2EXP_MAX_def, MOD_2EXP_def, GSYM BITS_ZERO3]
     \\ Cases_on `n`
-    >- SIMP_TAC std_ss [SYM LSB_ODD, LSB_def, BIT_def]
+    >- SIMP_TAC std_ss [SYM BIT0_ODD, BIT_def]
     \\ ONCE_REWRITE_TAC [GSYM lem]
-    \\ SIMP_TAC std_ss [GSYM BITS_ZERO3, SYM LSB_ODD, LSB_def,
-         GSYM BIT_BITS_THM, BIT_DIV2, DIV2_def]
-    \\ EQ_TAC \\ RW_TAC arith_ss [BIT_EXP_SUB1]
-    \\ Cases_on `x` \\ RW_TAC arith_ss []);
+    \\ SIMP_TAC std_ss
+          [GSYM BITS_ZERO3, SYM BIT0_ODD, GSYM BIT_BITS_THM, BIT_DIV2, DIV2_def]
+    \\ EQ_TAC
+    \\ RW_TAC arith_ss [BIT_EXP_SUB1]
+    \\ Cases_on `x` 
+    \\ RW_TAC arith_ss [])
 
 (* ------------------------------------------------------------------------- *)
 
 val LEAST_BIT_INTRO =
- (SIMP_RULE (srw_ss()) [] o SPEC `\i. BIT i n`)  whileTheory.LEAST_INTRO;
+   (SIMP_RULE (srw_ss()) [] o Q.SPEC `\i. BIT i n`)  whileTheory.LEAST_INTRO
 
-val LOWEST_SET_BIT = store_thm("LOWEST_SET_BIT",
-  `!n. ~(n = 0) ==>
-        (LOWEST_SET_BIT n =
-           if ODD n then 0 else 1 + LOWEST_SET_BIT (DIV2 n))`,
-  SRW_TAC [ARITH_ss] [LOWEST_SET_BIT_def,DIV2_def,ADD1]
-    \\ MATCH_MP_TAC LEAST_THM
-    \\ SRW_TAC [] [GSYM LSB_def,LSB_ODD]
-    >| [
+val LOWEST_SET_BIT = Q.store_thm("LOWEST_SET_BIT",
+   `!n. ~(n = 0) ==>
+        (LOWEST_SET_BIT n = if ODD n then 0 else 1 + LOWEST_SET_BIT (DIV2 n))`,
+   SRW_TAC [ARITH_ss] [LOWEST_SET_BIT_def, DIV2_def, ADD1]
+   \\ MATCH_MP_TAC LEAST_THM
+   \\ SRW_TAC [] [BIT0_ODD]
+   >| [
       Cases_on `(LEAST i. BIT i (n DIV 2)) = 0`
-        >| [
-          FULL_SIMP_TAC (srw_ss())
-            [DECIDE ``m < 1 ==> (m = 0)``,GSYM LSB_def,LSB_ODD],
-          IMP_RES_TAC (DECIDE ``~(a = 0) /\ m < a + 1 ==> (m - 1 < a)``)
-            \\ IMP_RES_TAC whileTheory.LESS_LEAST
-            \\ FULL_SIMP_TAC (srw_ss()) [BIT_DIV2]
-            \\ Cases_on `m = 0`
-            \\ FULL_SIMP_TAC (srw_ss()) [GSYM LSB_def,LSB_ODD,
-                 DECIDE ``~(m = 0) ==> (SUC (m - 1) = m)``]],
+      >- FULL_SIMP_TAC (srw_ss()) [DECIDE ``m < 1 ==> (m = 0)``, BIT0_ODD]
+      \\ IMP_RES_TAC (DECIDE ``~(a = 0) /\ m < a + 1 ==> (m - 1 < a)``)
+      \\ IMP_RES_TAC whileTheory.LESS_LEAST
+      \\ FULL_SIMP_TAC (srw_ss()) [BIT_DIV2]
+      \\ Cases_on `m = 0`
+      \\ FULL_SIMP_TAC (srw_ss())
+           [BIT0_ODD, DECIDE ``~(m = 0) ==> (SUC (m - 1) = m)``],
       SRW_TAC [] [GSYM ADD1, GSYM BIT_DIV2]
-        \\ MATCH_MP_TAC LEAST_BIT_INTRO
-        \\ `~(n DIV 2 = 0)` by (Cases_on `n = 1`
-              \\ FULL_SIMP_TAC arith_ss
-                   [(SIMP_RULE (srw_ss()) [DECIDE ``0 < n = ~(n = 0)``] o
-                     SPECL [`0`,`n`,`2`]) X_LT_DIV])
-        \\ METIS_TAC [BIT_LOG2]]);
+      \\ MATCH_MP_TAC LEAST_BIT_INTRO
+      \\ `~(n DIV 2 = 0)`
+      by (Cases_on `n = 1`
+          \\ FULL_SIMP_TAC arith_ss
+                [(SIMP_RULE (srw_ss()) [DECIDE ``0 < n = ~(n = 0)``] o
+                  Q.SPECL [`0`,`n`,`2`]) X_LT_DIV])
+      \\ METIS_TAC [BIT_LOG2]
+   ])
 
 val LOWEST_SET_BIT_compute = save_thm("LOWEST_SET_BIT_compute",
-let open numeralTheory
-    val rule = (GEN_ALL o SIMP_RULE (srw_ss())
-                 [DECIDE ``1 + n = SUC n``, numeral_eq, numeral_distrib,
-                  numeral_evenodd, numeral_div2])
-in
-  CONJ ((rule o SPEC `NUMERAL (BIT2 n)`) LOWEST_SET_BIT)
-       ((rule o SPEC `NUMERAL (BIT1 n)`) LOWEST_SET_BIT)
-end);
+   let
+      open numeralTheory
+      val rule = (GEN_ALL o SIMP_RULE (srw_ss())
+                   [DECIDE ``1 + n = SUC n``, numeral_eq, numeral_distrib,
+                     numeral_evenodd, numeral_div2])
+   in
+      CONJ ((rule o Q.SPEC `NUMERAL (BIT2 n)`) LOWEST_SET_BIT)
+           ((rule o Q.SPEC `NUMERAL (BIT1 n)`) LOWEST_SET_BIT)
+   end)
 
 (* ------------------------------------------------------------------------- *)
 
-val l2n_pow2_compute = store_thm("l2n_pow2_compute",
-  `(!p. l2n (2 ** p) [] = 0) /\
-   (!p h t. l2n (2 ** p) (h::t) =
-        MOD_2EXP p h + TIMES_2EXP p (l2n (2 ** p) t))`,
-  SRW_TAC [ARITH_ss] [l2n_def, TIMES_2EXP_def, MOD_2EXP_def]);
+val l2n_pow2_compute = Q.store_thm("l2n_pow2_compute",
+   `(!p. l2n (2 ** p) [] = 0) /\
+    (!p h t. l2n (2 ** p) (h::t) =
+             MOD_2EXP p h + TIMES_2EXP p (l2n (2 ** p) t))`,
+   SRW_TAC [ARITH_ss] [l2n_def, TIMES_2EXP_def, MOD_2EXP_def])
 
-val lem = (GEN_ALL o REWRITE_RULE [EXP] o SPECL [`n`,`0`] o
-           REWRITE_RULE [DECIDE ``1 < 2``] o SPEC `2`) EXP_BASE_LT_MONO;
+val lem = (GEN_ALL o REWRITE_RULE [EXP] o Q.SPECL [`n`,`0`] o
+           REWRITE_RULE [DECIDE ``1 < 2``] o Q.SPEC `2`) EXP_BASE_LT_MONO
 
-val n2l_pow2_compute = store_thm("n2l_pow2_compute",
-  `!p n. 0 < p ==>
-        (n2l (2 ** p) n =
-         let (q,r) = DIVMOD_2EXP p n in
-           if q = 0 then [r] else r::n2l (2 ** p) q)`,
-  SRW_TAC [] [Once n2l_def, DIVMOD_2EXP_def,
-              DECIDE ``x < 2 = (x = 0) \/ (x = 1)``]
-    \\ SRW_TAC [ARITH_ss] [LESS_DIV_EQ_ZERO]
-    \\ FULL_SIMP_TAC arith_ss [lem,DIV_0_IMP_LT]);
+val n2l_pow2_compute = Q.store_thm("n2l_pow2_compute",
+   `!p n. 0 < p ==>
+         (n2l (2 ** p) n =
+          let (q,r) = DIVMOD_2EXP p n in
+            if q = 0 then [r] else r::n2l (2 ** p) q)`,
+   SRW_TAC [] [Once n2l_def, DIVMOD_2EXP_def,
+               DECIDE ``x < 2 = (x = 0) \/ (x = 1)``]
+   \\ SRW_TAC [ARITH_ss] [LESS_DIV_EQ_ZERO]
+   \\ FULL_SIMP_TAC arith_ss [lem, DIV_0_IMP_LT])
 
 (* ------------------------------------------------------------------------- *)
 
-val _ = export_theory();
+val _ = export_theory()
