examples/ARM/v7/arm_stepScript.sml
@@ -798,8 +798,7 @@ val align_bx_bit = Q.store_thm("align_bx_bit",
    (!a:word32 n. (a || n2w n) ' 0 = a ' 0 \/ ODD n) /\
    (!a:word32 n. (a ?? n2w n) ' 0 = a ' 0 <> ODD n) /\
    (!a:word32 n. (a + n2w n) ' 0  = a ' 0 <> ODD n)`,
-  SRW_TAC [wordsLib.WORD_BIT_EQ_ss]
-    [WORD_ADD_BIT0, n2w_def, GSYM LSB_def, LSB_ODD]);
+  SRW_TAC [wordsLib.WORD_BIT_EQ_ss] [WORD_ADD_BIT0, n2w_def, BIT0_ODD]);
 
 val aligned_bx_thm = Q.store_thm("aligned_bx_thm",
   `!a:word32. aligned_bx a = (~a ' 0 ==> ~a ' 1)`,
